sepcomp-reserved/RG_interpolants.v
@@ -14,10 +14,10 @@ Require Import Globalenvs.
 Require Import sepcomp.mem_lemmas.
 Require Import sepcomp.core_semantics.
 
-Definition reserve_map_image (*{F1 V1 C1:Type} 
+Definition reserve_image (*{F1 V1 C1:Type} 
       (Sem: RelyGuaranteeSemantics (Genv.t F1 V1) C1 (list (ident * globdef F1 V1)))*)
-      (j:meminj) (r:reserve_map):reserve_map.
-  eapply Build_reserve_map with 
+      (j:meminj) (r:reserve'):reserve'.
+  eapply Build_reserve' with 
      (sort :=fun b2 => fun ofs => exists b1, exists delta2, j b1 = Some(b2, delta2) /\ r b1 (ofs - delta2)).
    admit. (*TODO -maybe use source-construction?*)
 Defined.
@@ -58,19 +58,19 @@ Parameter interpolate_IE: forall m1 m1' m2 j (Minj12 : Mem.inject j m1 m2) (Fwd1
                              (mem_wd m2 -> mem_wd m2').                                         
 *)
 Parameter interpolate_II: forall {F1 V1 C1 F2 V2 C2:Type}
-(Sem1 : RelyGuaranteeSemantics (Genv.t F1 V1) C1 (list (ident * globdef F1 V1)))
-(Sem2 : RelyGuaranteeSemantics (Genv.t F2 V2) C2 (list (ident * globdef F2 V2)))
+(Sem1 : EffectfulSemantics (Genv.t F1 V1) C1 (list (ident * globdef F1 V1)))
+(Sem2 : EffectfulSemantics (Genv.t F2 V2) C2 (list (ident * globdef F2 V2)))
                              m1 m2 j12 (MInj12 : Mem.inject j12 m1 m2) m1' (Fwd1: mem_forward m1 m1') j23 m3
                              (MInj23 : Mem.inject j23 m2 m3) m3' (Fwd3: mem_forward m3 m3')
                              j' (MInj13': Mem.inject j' m1' m3')
                              (InjIncr: inject_incr (compose_meminj j12 j23) j')
                              (InjSep: inject_separated (compose_meminj j12 j23) j' m1 m3)
                              (WD1: mem_wd m1) (WD1': mem_wd m1') (WD2: mem_wd m2) (WD3: mem_wd m3) (WD3' : mem_wd m3')
-                             st1 r r' st2
-                             (Rinc: reserve_map_incr r r')
-                             (Rsep13: reserve_map_separated r r' j' m1 m3)
-                             (Unch11': mem_unchanged_on (rely_left Sem1 r st1) m1 m1' )
-                             (Unch33': mem_unchanged_on (rely_right Sem1 (compose_meminj j12 j23) r st1) m3 m3')
+                             st1 (r r': reserve') st2
+                             (Rinc: reserve_incr r r')
+                             (Rsep13: reserve_separated r r' j' m1 m3)
+                             (Unch11': rely Sem1 r st1 m1 m1' )
+                             (Unch33': rely Sem1 (inject_reserve (compose_meminj j12 j23) r) st1 m3 m3')
 (*                             (Unch11': mem_unchanged_on (loc_unmapped (compose_meminj j12 j23)) m1 m1')
                              (Unch33': mem_unchanged_on (loc_out_of_reach (compose_meminj j12 j23) m1) m3 m3')*),
                  exists m2', exists j12', exists j23', j'=compose_meminj j12' j23' /\
@@ -78,14 +78,14 @@ Parameter interpolate_II: forall {F1 V1 C1 F2 V2 C2:Type}
                              Mem.inject j12' m1' m2' /\ mem_forward m2 m2' /\ Mem.inject j23' m2' m3' /\
                              inject_separated j12 j12' m1 m2 /\ inject_separated j23 j23' m2 m3 /\
                              (mem_wd m2 -> mem_wd m2') /\
-                             reserve_map_separated r r' j12' m1 m2 /\
+                             reserve_separated r r' j12' m1 m2 /\
                       exists r23, 
-                             mem_unchanged_on (rely_right Sem1 j12 r st1) m2 m2' /\
+                             rely Sem1 (inject_reserve j12 r) st1 m2 m2' /\
 (*                             mem_unchanged_on (loc_out_of_reach j12 m1) m2 m2' /\*)
-                             mem_unchanged_on (rely_left Sem2 r23 st2) m2 m2' /\ 
+                             rely Sem2 r23 st2 m2 m2' /\ 
 (*WAS:                             mem_unchanged_on (loc_unmapped j23) m2 m2' /\ *)
-                             mem_unchanged_on (rely_right Sem2 j23 r23 st2) m3 m3' /\
-                             r23 = reserve_map_image j12 r.
+                             rely Sem2 (inject_reserve j23 r23) st2 m3 m3' /\
+                             r23 = reserve_image j12 r.
 (*WAS:                             mem_unchanged_on (loc_out_of_reach j23 m2) m3 m3' /\*)                                
 
 End RGInterpolationAxioms.
